split interpret_call into several parts

L20/Interpret.v
@@ -14,27 +14,11 @@ Definition expr_result := L10.Interpret.expr_result.
 Definition stmt_result := L10.Interpret.stmt_result.
 Definition expr_error {type: Type} := @L10.Interpret.expr_error C type.
 
-Record calldag := {
-  cd_declmap:  string -> option decl;
-  cd_depthmap: string -> option nat;
-  cd_depthmap_ok:
-    forall name: string,
-      match cd_declmap name with
-      | None => True
-      | Some decl =>
-          match cd_depthmap name with
-          | None => False
-          | Some x =>
-              let _ := string_set_impl in
-              FSet.for_all (decl_callset decl)
-                           (fun callee => match cd_depthmap callee with
-                                          | None => false
-                                          | Some y => y <? x
-                                          end)
-               = true
-            end
-      end;
-}.
+Definition calldag := L10.Interpret.generic_calldag decl decl_callset.
+Definition cd_declmap {C decl_type callset} := @L10.Interpret.cd_declmap C decl_type callset.
+Definition cd_depthmap {C decl_type callset} := @L10.Interpret.cd_depthmap C decl_type callset.
+Definition cd_depthmap_ok {C decl_type callset} := @L10.Interpret.cd_depthmap_ok C decl_type callset.
+
 
 (** Initialize a map of local variables with argument names and argument values. *)
 Fixpoint bind_args (names: list string) (values: list uint256)
@@ -98,13 +82,14 @@ assert(HasName: let _ := string_set_impl in FSet.has (decl_callset this_decl) na
 }
 clear CallOk. cbn in HasName.
 assert (K := cd_depthmap_ok cd this_fun_name).
-rewrite this_decl_ok in K.
-rewrite current_fun_depth_ok in K.
+unfold cd_declmap in this_decl_ok. rewrite this_decl_ok in K.
+unfold cd_depthmap in current_fun_depth_ok. rewrite current_fun_depth_ok in K.
 cbn in K.
 rewrite FSet.for_all_ok in K.
 assert (L := K name HasName). clear K.
 subst call_depth_bound.
 apply lt_n_Sm_le in DepthOk.
+unfold cd_depthmap in Edepth.
 rewrite Edepth in L.
 destruct current_fun_depth. { discriminate. }
 rewrite Nat.leb_le in L.
@@ -134,8 +119,10 @@ Local Lemma fun_ctx_descend_helper {cd: calldag}
   cd_depthmap cd name <> None.
 Proof.
 assert (D := cd_depthmap_ok cd name).
+unfold cd_declmap in Edecl.
 rewrite Edecl in D.
 intro H.
+unfold cd_depthmap in H.
 rewrite H in D.
 exact D.
 Qed.
@@ -186,6 +173,344 @@ Definition map_lookup {Value} (m: string_map Value) := let _ := string_map_impl 
 Definition map_insert {Value} (m: string_map Value) := let _ := string_map_impl in Map.insert m.
 Definition map_remove {Value} (m: string_map Value) := let _ := string_map_impl in Map.remove m.
 
+Fixpoint interpret_expr {bigger_call_depth_bound smaller_call_depth_bound: nat}
+                        (Ebound: bigger_call_depth_bound = S smaller_call_depth_bound)
+                        {cd: calldag}
+                        (fc: fun_ctx cd bigger_call_depth_bound)
+                        (do_call: forall
+                                      (fc': fun_ctx cd smaller_call_depth_bound)
+                                      (world: world_state)
+                                      (arg_values: list uint256),
+                                    world_state * expr_result uint256)
+                        (builtins: string -> option L10.Interpret.builtin)
+                        (world: world_state)
+                        (loc: string_map uint256)
+                        (e: expr)
+                        (CallOk: let _ := string_set_impl in 
+                                   FSet.is_subset (expr_callset e)
+                                                  (decl_callset (fun_decl fc))
+                                   = true)
+{struct e}
+: world_state * expr_result uint256
+:= let fix interpret_expr_list (world: world_state)
+                               (loc: string_map uint256)
+                               (e: list expr)
+                               (CallOk: let _ := string_set_impl in 
+                                        FSet.is_subset (expr_list_callset e)
+                                                       (decl_callset (fun_decl fc))
+                                        = true)
+      {struct e}
+      : world_state * expr_result (list uint256)
+      := match e as e' return e = e' -> _ with
+         | nil => fun _ => (world, L10.Interpret.ExprSuccess _ nil)
+         | (h :: t)%list => fun E =>
+             let (world', result_h) := interpret_expr Ebound fc do_call builtins
+                                                      world loc h
+                                                      (callset_descend_head E CallOk)
+             in match result_h with
+                | L10.Interpret.ExprAbort _ ab => (world', L10.Interpret.ExprAbort _ ab)
+                | L10.Interpret.ExprSuccess _ x =>
+                   let (world'', result_t) := interpret_expr_list world' loc t
+                                                                  (callset_descend_tail E CallOk)
+                   in (world'', match result_t with
+                                | L10.Interpret.ExprAbort _ _ => result_t
+                                | L10.Interpret.ExprSuccess _ y => 
+                                    L10.Interpret.ExprSuccess _ (x :: y)%list
+                                end)
+                 end
+         end eq_refl
+    in match e as e' return e = e' -> _ with
+       | Const val => fun _ => (world, L10.Interpret.ExprSuccess _ val)
+       | LocalVar name => fun _ =>
+           (world, match map_lookup loc name with
+                   | Some val => L10.Interpret.ExprSuccess _ val
+                   | None => expr_error "Local variable not found"
+                   end)
+       | StorageVar name => fun _ => 
+           (world, match storage_lookup world name with
+                   | Some val => L10.Interpret.ExprSuccess _ val
+                   | None => expr_error "Storage variable not found"
+                   end)
+       | UnOp op a => fun E =>
+           let (world', result) := interpret_expr Ebound fc do_call builtins
+                                                  world loc a
+                                                  (callset_descend_unop E CallOk)
+           in (world', match result with
+                       | L10.Interpret.ExprSuccess _ val => L10.Interpret.interpret_unop op val
+                       | L10.Interpret.ExprAbort _ _ => result
+                       end)
+       | BinOp op a b => fun E =>
+           let (world', result_a) := interpret_expr Ebound fc do_call builtins
+                                                    world loc a
+                                                    (callset_descend_binop_left E CallOk)
+           in match result_a with
+           | L10.Interpret.ExprAbort _ _ => (world', result_a)
+           | L10.Interpret.ExprSuccess _ x =>
+             let (world'', result_b) := interpret_expr Ebound fc do_call builtins
+                                                       world' loc b
+                                                       (callset_descend_binop_right E CallOk)
+             in (world'', match result_b with
+                          | L10.Interpret.ExprAbort _ _ => result_b
+                          | L10.Interpret.ExprSuccess _ y => L10.Interpret.interpret_binop op x y
+                          end)
+           end
+       | IfThenElse cond yes no => fun E =>
+           let (world', result_cond) := interpret_expr Ebound fc do_call builtins
+                                                       world loc cond
+                                                       (callset_descend_if_cond E CallOk)
+           in match result_cond with
+              | L10.Interpret.ExprAbort _ _ => (world', result_cond)
+              | L10.Interpret.ExprSuccess _ cond_value =>
+                  if (Z_of_uint256 cond_value =? 0)%Z
+                    then interpret_expr Ebound fc do_call builtins
+                                        world' loc no
+                                        (callset_descend_if_else E CallOk)
+                    else interpret_expr Ebound fc do_call builtins
+                                        world' loc yes
+                                        (callset_descend_if_then E CallOk)
+              end
+       | LogicalAnd a b => fun E =>
+           let (world', result_a) := interpret_expr Ebound fc do_call builtins
+                                                    world loc a
+                                                    (callset_descend_and_left E CallOk)
+           in match result_a with
+              | L10.Interpret.ExprAbort _ _ => (world', result_a)
+              | L10.Interpret.ExprSuccess _ a_value =>
+                  if (Z_of_uint256 a_value =? 0)%Z
+                    then (world', result_a)
+                    else interpret_expr Ebound fc do_call builtins
+                                        world' loc b
+                                        (callset_descend_and_right E CallOk)
+              end
+       | LogicalOr a b => fun E =>
+           let (world', result_a) := interpret_expr Ebound fc do_call builtins
+                                                    world loc a
+                                                    (callset_descend_or_left E CallOk)
+           in match result_a with
+              | L10.Interpret.ExprAbort _ msg => (world', result_a)
+              | L10.Interpret.ExprSuccess _ a_value =>
+                  if (Z_of_uint256 a_value =? 0)%Z
+                    then interpret_expr Ebound fc do_call builtins
+                                        world' loc b
+                                        (callset_descend_or_right E CallOk)
+                    else (world', result_a)
+              end
+       | PrivateCall name args => fun E =>
+           let (world', result_args) :=
+             interpret_expr_list world loc args
+                                 (callset_descend_args E CallOk)
+           in match result_args with
+              | L10.Interpret.ExprAbort _ ab => (world', L10.Interpret.ExprAbort _ ab)
+              | L10.Interpret.ExprSuccess _ arg_values =>
+                  match fun_ctx_descend fc CallOk Ebound E with
+                  | None => (* can't resolve the function, maybe it's a builtin *)
+                            (world', expr_error "can't resolve function name")
+                  | Some new_fc => do_call new_fc world' arg_values
+                  end
+              end
+       | BuiltinCall name args => fun E =>
+           let (world', result_args) :=
+             interpret_expr_list world loc args
+                                 (callset_descend_builtin_args E CallOk)
+           in match result_args with
+              | L10.Interpret.ExprAbort _ ab => (world', L10.Interpret.ExprAbort _ ab)
+              | L10.Interpret.ExprSuccess _ arg_values =>
+                match builtins name with
+                | Some (existT _ arity b) =>
+                   (if (arity =? List.length arg_values)%nat as arity_ok 
+                    return _ = arity_ok -> _
+                        then fun Earity =>
+                               L10.Interpret.call_builtin arg_values Earity (b world')
+                        else fun _ => (world', expr_error "builtin with wrong arity"))
+                      eq_refl
+                | None => (world', expr_error "can't resolve function name")
+                end
+              end
+       end eq_refl.
+
+Definition interpret_small_stmt {bigger_call_depth_bound smaller_call_depth_bound: nat}
+                                (Ebound: bigger_call_depth_bound = S smaller_call_depth_bound)
+                                {cd: calldag}
+                                (fc: fun_ctx cd bigger_call_depth_bound)
+                                (do_call: forall
+                                              (fc': fun_ctx cd smaller_call_depth_bound)
+                                              (world: world_state)
+                                              (arg_values: list uint256),
+                                            world_state * expr_result uint256)
+                                (builtins: string -> option L10.Interpret.builtin)
+                                (world: world_state)
+                                (loc: string_map uint256)
+                                (s: small_stmt)
+                                (CallOk: let _ := string_set_impl in 
+                                         FSet.is_subset (small_stmt_callset s)
+                                                        (decl_callset (fun_decl fc))
+                                         = true)
+: world_state * string_map uint256 * stmt_result uint256
+:= match s as s' return s = s' -> _ with
+   | Pass     => fun _ => (world, loc, L10.Interpret.StmtSuccess _)
+   | Abort ab => fun _ => (world, loc, L10.Interpret.StmtAbort _ ab)
+   | Return e => fun E =>
+        let (world', result) := interpret_expr Ebound fc do_call builtins
+                                               world loc e
+                                               (callset_descend_return E CallOk)
+        in (world', loc, match result with
+                         | L10.Interpret.ExprSuccess _ value =>
+                              L10.Interpret.StmtReturnFromFunction _ value
+                         | L10.Interpret.ExprAbort _ ab =>
+                              L10.Interpret.StmtAbort _ ab
+                         end)
+   | Raise e => fun E =>
+        let (world', result) := interpret_expr Ebound fc do_call builtins
+                                               world loc e
+                                               (callset_descend_raise E CallOk)
+        in (world', loc, L10.Interpret.StmtAbort _
+                           (match result with
+                            | L10.Interpret.ExprSuccess _ value =>
+                                L10.Interpret.AbortException value
+                            | L10.Interpret.ExprAbort _ ab => ab
+                            end))
+   | Assign lhs rhs => fun E =>
+        let (world', result) := interpret_expr Ebound fc do_call builtins
+                                               world loc rhs
+                                               (callset_descend_assign_rhs E CallOk)
+        in L10.Interpret.do_assign world' loc lhs result
+   | ExprStmt e => fun E =>
+                   let (world', result) := interpret_expr Ebound fc do_call builtins
+                                                          world loc e
+                                                          (callset_descend_expr_stmt E CallOk)
+                   in (world', loc, match result with
+                                    | L10.Interpret.ExprSuccess _ a =>
+                                        L10.Interpret.StmtSuccess _
+                                    | L10.Interpret.ExprAbort _ ab =>
+                                        L10.Interpret.StmtAbort _ ab
+                                    end)
+   end eq_refl.
+
+Fixpoint interpret_stmt {bigger_call_depth_bound smaller_call_depth_bound: nat}
+                        (Ebound: bigger_call_depth_bound = S smaller_call_depth_bound)
+                        {cd: calldag}
+                        (fc: fun_ctx cd bigger_call_depth_bound)
+                        (do_call: forall
+                                      (fc': fun_ctx cd smaller_call_depth_bound)
+                                      (world: world_state)
+                                      (arg_values: list uint256),
+                                    world_state * expr_result uint256)
+                        (builtins: string -> option L10.Interpret.builtin)
+                        (world: world_state)
+                        (loc: string_map uint256)
+                        (s: stmt)
+                        (CallOk: let _ := string_set_impl in 
+                                 FSet.is_subset (stmt_callset s)
+                                                (decl_callset (fun_decl fc)) = true)
+ {struct s}
+ : world_state * string_map uint256 * stmt_result uint256
+ := match s as s' return s = s' -> _ with
+    | Semicolon a b => fun E =>
+         let '(world', loc', result_a) :=
+                interpret_stmt Ebound fc do_call builtins
+                               world loc a
+                               (callset_descend_semicolon_left E CallOk) in
+         match result_a with
+         | L10.Interpret.StmtSuccess _ =>
+             interpret_stmt Ebound fc do_call builtins
+                            world' loc' b
+                            (callset_descend_semicolon_right E CallOk)
+         | _ => (world', loc', result_a)
+         end
+    | SmallStmt ss => fun E => interpret_small_stmt Ebound fc do_call builtins
+                                                    world loc ss
+                                                    (callset_descend_small_stmt E CallOk)
+    | LocalVarDecl name init scope => fun E =>
+         match map_lookup loc name with
+         | Some _ => (world, loc,
+                        L10.Interpret.StmtAbort _
+                          (L10.Interpret.AbortError "local variable already exists"))
+         | None =>
+           let '(world', result) :=
+                  interpret_expr Ebound fc do_call builtins
+                                 world loc init
+                                 (callset_descend_var_init E CallOk)
+           in match result with
+              | L10.Interpret.ExprSuccess _ value =>
+                  let '(world2, loc2, result2) :=
+                    interpret_stmt Ebound fc do_call builtins
+                                   world (map_insert loc name value) scope
+                                   (callset_descend_var_scope E CallOk)
+                  in (world2, map_remove loc2 name, result2)
+              | L10.Interpret.ExprAbort _ ab =>
+                  (world', loc, L10.Interpret.StmtAbort _ ab)
+              end
+         end
+    | IfElseStmt cond yes no => fun E => 
+        let (world', result_cond) := interpret_expr
+                                       Ebound fc do_call builtins
+                                       world loc cond
+                                       (callset_descend_stmt_if_cond E CallOk)
+        in match result_cond with
+           | L10.Interpret.ExprAbort _ ab => (world', loc, L10.Interpret.StmtAbort _ ab)
+           | L10.Interpret.ExprSuccess _ cond_value =>
+               if (Z_of_uint256 cond_value =? 0)%Z
+                 then interpret_stmt Ebound fc do_call builtins
+                                     world' loc no
+                                     (callset_descend_stmt_if_else E CallOk)
+                 else interpret_stmt Ebound fc do_call builtins
+                                     world' loc yes
+                                     (callset_descend_stmt_if_then E CallOk)
+           end
+    | Loop var start count fc_body => fun E =>
+        let (world', result_start) :=
+              interpret_expr Ebound fc do_call builtins
+                             world loc start
+                             (callset_descend_loop_start E CallOk)
+        in match result_start with
+           | L10.Interpret.ExprAbort _ ab => (world', loc, L10.Interpret.StmtAbort _ ab)
+           | L10.Interpret.ExprSuccess _ start_value =>
+              let fix interpret_loop_rec (world: world_state)
+                                         (loc: string_map uint256)
+                                         (cursor: Z)
+                                         (countdown: nat)
+                                         (name: string)
+                                         (CallOk: let _ := string_set_impl in 
+                                                  FSet.is_subset (stmt_callset fc_body)
+                                                                 (decl_callset (fun_decl fc)) = true)
+                 {struct countdown}
+                 : world_state * string_map uint256 * stmt_result uint256
+                 := match countdown with
+                    | O => (world, loc, L10.Interpret.StmtSuccess _)
+                    | S new_countdown =>
+                          let loc' := map_insert loc name (uint256_of_Z cursor) in
+                          let '(world', loc'', result) :=
+                                interpret_stmt Ebound fc do_call builtins world loc' fc_body CallOk
+                          in match result with
+                             | L10.Interpret.StmtSuccess _
+                             | L10.Interpret.StmtAbort _ L10.Interpret.AbortContinue =>
+                                 interpret_loop_rec world' loc''
+                                                    (Z.succ cursor) new_countdown name CallOk
+                             | L10.Interpret.StmtAbort _ L10.Interpret.AbortBreak =>
+                                 (world', loc'', L10.Interpret.StmtSuccess _)
+                             | _ => (world', loc'', result)
+                             end
+                    end
+               in match map_lookup loc var with
+               | Some _ => (world', loc,
+                             L10.Interpret.StmtAbort _
+                               (L10.Interpret.AbortError "loop var already exists"))
+               | None => let count_z := Z_of_uint256 count in
+                         let count_nat := Z.to_nat count_z in
+                         let start_z := Z_of_uint256 start_value in
+                         let last := (start_z + count_z - 1)%Z in
+                         if (Z_of_uint256 (uint256_of_Z last) =? last)%Z
+                           then
+                             interpret_loop_rec
+                               world' loc start_z count_nat var
+                               (callset_descend_loop_body E CallOk)
+                           else (world, loc,
+                                  L10.Interpret.StmtAbort _
+                                    (L10.Interpret.AbortError "loop range overflows"))
+               end
+           end
+    end eq_refl.
+
 Fixpoint interpret_call {call_depth_bound: nat}
                         {cd: calldag}
                         (builtins: string -> option L10.Interpret.builtin)
@@ -194,299 +519,17 @@ Fixpoint interpret_call {call_depth_bound: nat}
                         (arg_values: list uint256)
 {struct call_depth_bound}
 : world_state * expr_result uint256
-:= let fix interpret_expr (world: world_state)
-                          (loc: string_map uint256)
-                          (e: expr)
-                          (CallOk: let _ := string_set_impl in 
-                                     FSet.is_subset (expr_callset e)
-                                                    (decl_callset (fun_decl fc))
-                                     = true)
-      {struct e}
-      : world_state * expr_result uint256
-      := let fix interpret_expr_list (world: world_state)
-                                     (loc: string_map uint256)
-                                     (e: list expr)
-                                     (CallOk: let _ := string_set_impl in 
-                                              FSet.is_subset (expr_list_callset e)
-                                                             (decl_callset (fun_decl fc))
-                                              = true)
-            {struct e}
-            : world_state * expr_result (list uint256)
-            := match e as e' return e = e' -> _ with
-               | nil => fun _ => (world, L10.Interpret.ExprSuccess _ nil)
-               | (h :: t)%list => fun E =>
-                   let (world', result_h) := interpret_expr world loc h
-                                                            (callset_descend_head E CallOk)
-                   in match result_h with
-                      | L10.Interpret.ExprAbort _ ab => (world', L10.Interpret.ExprAbort _ ab)
-                      | L10.Interpret.ExprSuccess _ x =>
-                         let (world'', result_t) := interpret_expr_list world' loc t
-                                                                        (callset_descend_tail E CallOk)
-                         in (world'', match result_t with
-                                      | L10.Interpret.ExprAbort _ _ => result_t
-                                      | L10.Interpret.ExprSuccess _ y => 
-                                          L10.Interpret.ExprSuccess _ (x :: y)%list
-                                      end)
-                       end
-               end eq_refl
-         in match call_depth_bound as call_depth_bound' return _ = call_depth_bound' -> _ with
-            | O => fun Ebound => False_rect _ (Nat.nlt_0_r (fun_depth fc)
-                                                           (eq_ind _ _ (fun_bound_ok fc) _ Ebound))
-            | S new_call_depth_bound => fun Ebound =>
-
-                 match e as e' return e = e' -> _ with
-                 | Const val => fun _ => (world, L10.Interpret.ExprSuccess _ val)
-                 | LocalVar name => fun _ =>
-                     (world, match map_lookup loc name with
-                             | Some val => L10.Interpret.ExprSuccess _ val
-                             | None => expr_error "Local variable not found"
-                             end)
-                 | StorageVar name => fun _ => 
-                     (world, match storage_lookup world name with
-                             | Some val => L10.Interpret.ExprSuccess _ val
-                             | None => expr_error "Storage variable not found"
-                             end)
-                 | UnOp op a => fun E =>
-                     let (world', result) := interpret_expr world loc a
-                                                            (callset_descend_unop E CallOk)
-                     in (world', match result with
-                                 | L10.Interpret.ExprSuccess _ val => L10.Interpret.interpret_unop op val
-                                 | L10.Interpret.ExprAbort _ _ => result
-                                 end)
-                 | BinOp op a b => fun E =>
-                     let (world', result_a) := interpret_expr world loc a
-                                                              (callset_descend_binop_left E CallOk)
-                     in match result_a with
-                     | L10.Interpret.ExprAbort _ _ => (world', result_a)
-                     | L10.Interpret.ExprSuccess _ x =>
-                       let (world'', result_b) := interpret_expr world' loc b
-                                                                 (callset_descend_binop_right E CallOk)
-                       in (world'', match result_b with
-                                    | L10.Interpret.ExprAbort _ _ => result_b
-                                    | L10.Interpret.ExprSuccess _ y => L10.Interpret.interpret_binop op x y
-                                    end)
-                     end
-                 | IfThenElse cond yes no => fun E =>
-                     let (world', result_cond) := interpret_expr world loc cond
-                                                                 (callset_descend_if_cond E CallOk)
-                     in match result_cond with
-                        | L10.Interpret.ExprAbort _ _ => (world', result_cond)
-                        | L10.Interpret.ExprSuccess _ cond_value =>
-                            if (Z_of_uint256 cond_value =? 0)%Z
-                              then interpret_expr world' loc no
-                                                  (callset_descend_if_else E CallOk)
-                              else interpret_expr world' loc yes
-                                                  (callset_descend_if_then E CallOk)
-                        end
-                 | LogicalAnd a b => fun E =>
-                     let (world', result_a) := interpret_expr world loc a
-                                                              (callset_descend_and_left E CallOk)
-                     in match result_a with
-                        | L10.Interpret.ExprAbort _ _ => (world', result_a)
-                        | L10.Interpret.ExprSuccess _ a_value =>
-                            if (Z_of_uint256 a_value =? 0)%Z
-                              then (world', result_a)
-                              else interpret_expr world' loc b
-                                                  (callset_descend_and_right E CallOk)
-                        end
-                 | LogicalOr a b => fun E =>
-                     let (world', result_a) := interpret_expr world loc a
-                                                              (callset_descend_or_left E CallOk)
-                     in match result_a with
-                        | L10.Interpret.ExprAbort _ msg => (world', result_a)
-                        | L10.Interpret.ExprSuccess _ a_value =>
-                            if (Z_of_uint256 a_value =? 0)%Z
-                              then interpret_expr world' loc b
-                                                  (callset_descend_or_right E CallOk)
-                              else (world', result_a)
-                        end
-                 | PrivateCall name args => fun E =>
-                     let (world', result_args) :=
-                       interpret_expr_list world loc args
-                                           (callset_descend_args E CallOk)
-                     in match result_args with
-                        | L10.Interpret.ExprAbort _ ab => (world', L10.Interpret.ExprAbort _ ab)
-                        | L10.Interpret.ExprSuccess _ arg_values =>
-                            match fun_ctx_descend fc CallOk Ebound E with
-                            | None => (* can't resolve the function, maybe it's a builtin *)
-                                      (world', expr_error "can't resolve function name")
-                            | Some new_fc => interpret_call builtins new_fc world' arg_values
-                            end
-                        end
-                 | BuiltinCall name args => fun E =>
-                     let (world', result_args) :=
-                       interpret_expr_list world loc args
-                                           (callset_descend_builtin_args E CallOk)
-                     in match result_args with
-                        | L10.Interpret.ExprAbort _ ab => (world', L10.Interpret.ExprAbort _ ab)
-                        | L10.Interpret.ExprSuccess _ arg_values =>
-                          match builtins name with
-                          | Some (existT _ arity b) =>
-                             (if (arity =? List.length arg_values)%nat as arity_ok 
-                              return _ = arity_ok -> _
-                                  then fun Earity =>
-                                         L10.Interpret.call_builtin arg_values Earity (b world')
-                                  else fun _ => (world', expr_error "builtin with wrong arity"))
-                                eq_refl
-                          | None => (world', expr_error "can't resolve function name")
-                          end
-                        end
-                 end eq_refl
-         end eq_refl
-     in let interpret_small_stmt (world: world_state)
-                                 (loc: string_map uint256)
-                                 (s: small_stmt)
-                                 (CallOk: let _ := string_set_impl in 
-                                          FSet.is_subset (small_stmt_callset s)
-                                                         (decl_callset (fun_decl fc))
-                                           =
-                                          true)
-        : world_state * string_map uint256 * stmt_result uint256
-        := match s as s' return s = s' -> _ with
-           | Pass     => fun _ => (world, loc, L10.Interpret.StmtSuccess _)
-           | Abort ab => fun _ => (world, loc, L10.Interpret.StmtAbort _ ab)
-           | Return e => fun E =>
-                let (world', result) := interpret_expr world loc e
-                                                       (callset_descend_return E CallOk)
-                in (world', loc, match result with
-                                 | L10.Interpret.ExprSuccess _ value =>
-                                      L10.Interpret.StmtReturnFromFunction _ value
-                                 | L10.Interpret.ExprAbort _ ab =>
-                                      L10.Interpret.StmtAbort _ ab
-                                 end)
-           | Raise e => fun E =>
-                let (world', result) := interpret_expr world loc e
-                                                       (callset_descend_raise E CallOk)
-                in (world', loc, L10.Interpret.StmtAbort _
-                                   (match result with
-                                    | L10.Interpret.ExprSuccess _ value =>
-                                        L10.Interpret.AbortException value
-                                    | L10.Interpret.ExprAbort _ ab => ab
-                                    end))
-           | Assign lhs rhs => fun E =>
-                let (world', result) := interpret_expr world loc rhs
-                                                       (callset_descend_assign_rhs E CallOk)
-                in L10.Interpret.do_assign world' loc lhs result
-           | ExprStmt e => fun E =>
-                           let (world', result) := interpret_expr world loc e
-                                                   (callset_descend_expr_stmt E CallOk)
-                           in (world', loc, match result with
-                                            | L10.Interpret.ExprSuccess _ a =>
-                                                L10.Interpret.StmtSuccess _
-                                            | L10.Interpret.ExprAbort _ ab =>
-                                                L10.Interpret.StmtAbort _ ab
-                                            end)
-           end eq_refl
-     in let fix interpret_stmt (world: world_state)
-                               (loc: string_map uint256)
-                               (s: stmt)
-                               (CallOk: let _ := string_set_impl in 
-                                        FSet.is_subset (stmt_callset s)
-                                                       (decl_callset (fun_decl fc)) = true)
-           {struct s}
-           : world_state * string_map uint256 * stmt_result uint256
-           := match s as s' return s = s' -> _ with
-              | Semicolon a b => fun E =>
-                   let '(world', loc', result_a) :=
-                          interpret_stmt world loc a
-                                         (callset_descend_semicolon_left E CallOk) in
-                   match result_a with
-                   | L10.Interpret.StmtSuccess _ =>
-                       interpret_stmt world' loc' b
-                                      (callset_descend_semicolon_right E CallOk)
-                   | _ => (world', loc', result_a)
-                   end
-              | SmallStmt ss => fun E => interpret_small_stmt world loc ss
-                                                     (callset_descend_small_stmt E CallOk)
-              | LocalVarDecl name init scope => fun E =>
-                   match map_lookup loc name with
-                   | Some _ => (world, loc,
-                                  L10.Interpret.StmtAbort _
-                                    (L10.Interpret.AbortError "local variable already exists"))
-                   | None =>
-                     let '(world', result) :=
-                            interpret_expr world loc init
-                                           (callset_descend_var_init E CallOk)
-                     in match result with
-                        | L10.Interpret.ExprSuccess _ value =>
-                            let '(world2, loc2, result2) :=
-                              interpret_stmt world (map_insert loc name value) scope
-                                             (callset_descend_var_scope E CallOk)
-                            in (world2, map_remove loc2 name, result2)
-                        | L10.Interpret.ExprAbort _ ab =>
-                            (world', loc, L10.Interpret.StmtAbort _ ab)
-                        end
-                   end
-              | IfElseStmt cond yes no => fun E => 
-                  let (world', result_cond) := interpret_expr
-                                                 world loc cond
-                                                 (callset_descend_stmt_if_cond E CallOk)
-                  in match result_cond with
-                     | L10.Interpret.ExprAbort _ ab => (world', loc, L10.Interpret.StmtAbort _ ab)
-                     | L10.Interpret.ExprSuccess _ cond_value =>
-                         if (Z_of_uint256 cond_value =? 0)%Z
-                           then interpret_stmt world' loc no
-                                               (callset_descend_stmt_if_else E CallOk)
-                           else interpret_stmt world' loc yes
-                                               (callset_descend_stmt_if_then E CallOk)
-                     end
-              | Loop var start count fc_body => fun E =>
-                  let (world', result_start) :=
-                        interpret_expr world loc start
-                                       (callset_descend_loop_start E CallOk)
-                  in match result_start with
-                     | L10.Interpret.ExprAbort _ ab => (world', loc, L10.Interpret.StmtAbort _ ab)
-                     | L10.Interpret.ExprSuccess _ start_value =>
-                        let fix interpret_loop_rec (world: world_state)
-                                                   (loc: string_map uint256)
-                                                   (cursor: Z)
-                                                   (countdown: nat)
-                                                   (name: string)
-                                                   (CallOk: let _ := string_set_impl in 
-                                                            FSet.is_subset (stmt_callset fc_body)
-                                                                           (decl_callset (fun_decl fc)) = true)
-                           {struct countdown}
-                           : world_state * string_map uint256 * stmt_result uint256
-                           := match countdown with
-                              | O => (world, loc, L10.Interpret.StmtSuccess _)
-                              | S new_countdown =>
-                                    let loc' := map_insert loc name (uint256_of_Z cursor) in
-                                    let '(world', loc'', result) := interpret_stmt world loc' fc_body CallOk
-                                    in match result with
-                                       | L10.Interpret.StmtSuccess _
-                                       | L10.Interpret.StmtAbort _ L10.Interpret.AbortContinue =>
-                                           interpret_loop_rec world' loc''
-                                                              (Z.succ cursor) new_countdown name CallOk
-                                       | L10.Interpret.StmtAbort _ L10.Interpret.AbortBreak =>
-                                           (world', loc'', L10.Interpret.StmtSuccess _)
-                                       | _ => (world', loc'', result)
-                                       end
-                              end
-                         in match map_lookup loc var with
-                         | Some _ => (world', loc,
-                                       L10.Interpret.StmtAbort _
-                                         (L10.Interpret.AbortError "loop var already exists"))
-                         | None => let count_z := Z_of_uint256 count in
-                                   let count_nat := Z.to_nat count_z in
-                                   let start_z := Z_of_uint256 start_value in
-                                   let last := (start_z + count_z - 1)%Z in
-                                   if (Z_of_uint256 (uint256_of_Z last) =? last)%Z
-                                     then
-                                       interpret_loop_rec
-                                         world' loc start_z count_nat var
-                                         (callset_descend_loop_body E CallOk)
-                                     else (world, loc,
-                                            L10.Interpret.StmtAbort _
-                                              (L10.Interpret.AbortError "loop range overflows"))
-                         end
-                     end
-              end eq_refl
-     in match fun_decl fc as d return _ = d -> _ with
+:= match call_depth_bound as call_depth_bound' return _ = call_depth_bound' -> _ with
+   | O => fun Ebound => False_rect _ (Nat.nlt_0_r (fun_depth fc)
+                                                  (eq_ind _ _ (fun_bound_ok fc) _ Ebound))
+   | S new_call_depth_bound => fun Ebound =>
+        match fun_decl fc as d return _ = d -> _ with
         | FunDecl _ arg_names body => fun E =>
             match bind_args arg_names arg_values with
             | inl err => (world, expr_error err)
             | inr loc =>
-                let '(world', loc', result) := interpret_stmt world loc body 
+                let '(world', loc', result) := interpret_stmt Ebound fc (interpret_call builtins)
+                                                              builtins world loc body 
                                                               (interpret_call_helper E)
                 in (world', match result with
                             | L10.Interpret.StmtSuccess _ => L10.Interpret.ExprSuccess _ zero256
@@ -495,7 +538,8 @@ Fixpoint interpret_call {call_depth_bound: nat}
                             end)
             end
         | _ => fun _ => (world, expr_error "a declaration is found but it's not a function")
-        end eq_refl.
+        end eq_refl
+   end eq_refl.
 
 Local Lemma make_fun_ctx_helper {cd: calldag}
                           {name: string}
@@ -505,7 +549,10 @@ Local Lemma make_fun_ctx_helper {cd: calldag}
   False.
 Proof.
 assert (W := cd_depthmap_ok cd name).
-rewrite Ed in W. rewrite Edepth in W. exact W.
+unfold cd_declmap in Ed.
+rewrite Ed in W.
+unfold cd_depthmap in Edepth.
+rewrite Edepth in W. exact W.
 Qed.
 
 Definition make_fun_ctx_and_bound (cd: calldag)
