L10/Interpret.v
@@ -47,8 +47,8 @@ Definition interpret_binop (op: binop) (a b: uint256)
    | None => expr_error "arithmetic error"
    end.
 
-Record calldag := {
-  cd_declmap:  string -> option decl;
+Record generic_calldag (decl_type: Type) (callset: decl_type -> string_set) := {
+  cd_declmap:  string -> option decl_type;
   cd_depthmap: string -> option nat;
   cd_depthmap_ok:
     forall name: string,
@@ -59,7 +59,7 @@ Record calldag := {
           | None => False
           | Some x =>
               let _ := string_set_impl in
-              FSet.for_all (decl_callset decl)
+              FSet.for_all (callset decl)
                            (fun callee => match cd_depthmap callee with
                                           | None => false
                                           | Some y => y <? x
@@ -68,6 +68,11 @@ Record calldag := {
             end
       end;
 }.
+Arguments cd_declmap {decl_type callset}.
+Arguments cd_depthmap {decl_type callset}.
+Arguments cd_depthmap_ok {decl_type callset}.
+
+Definition calldag := generic_calldag decl decl_callset.
 
 (** Initialize a map of local variables with argument names and argument values. *)
 Fixpoint bind_args (names: list string) (values: list uint256)
@@ -292,6 +297,479 @@ Definition call_builtin {arity: nat}
 : world_state * expr_result uint256
 := fst (nary_call callable args (Nat.eq_le_incl _ _ (proj1 (Nat.eqb_eq _ _) ArityOk))).
 
+Fixpoint interpret_expr {bigger_call_depth_bound smaller_call_depth_bound: nat}
+                        (Ebound: bigger_call_depth_bound = S smaller_call_depth_bound)
+                        {cd: calldag}
+                        (fc: fun_ctx cd bigger_call_depth_bound)
+                        (do_call: forall
+                                      (fc': fun_ctx cd smaller_call_depth_bound)
+                                      (world: world_state)
+                                      (arg_values: list uint256),
+                                    world_state * expr_result uint256)
+                        (builtins: string -> option builtin)
+                        (world: world_state)
+                        (loc: string_map uint256)
+                        (e: expr)
+                        (CallOk: let _ := string_set_impl in 
+                                 FSet.is_subset (expr_callset e)
+                                                (decl_callset (fun_decl fc))
+                                 = true)
+{struct e}
+: world_state * expr_result uint256
+:= let fix interpret_expr_list (world: world_state)
+                           (loc: string_map uint256)
+                           (e: list expr)
+                           (CallOk: let _ := string_set_impl in 
+                                    FSet.is_subset (expr_list_callset e)
+                                                   (decl_callset (fun_decl fc))
+                                    = true)
+  {struct e}
+  : world_state * expr_result (list uint256)
+  := match e as e' return e = e' -> _ with
+     | nil => fun _ => (world, ExprSuccess nil)
+     | (h :: t)%list => fun E =>
+         let (world', result_h) := interpret_expr Ebound fc do_call builtins
+                                                  world loc h
+                                                  (callset_descend_head E CallOk)
+         in match result_h with
+            | ExprAbort ab => (world', ExprAbort ab)
+            | ExprSuccess x =>
+               let (world'', result_t) := interpret_expr_list world' loc t
+                                                              (callset_descend_tail E CallOk)
+               in (world'', match result_t with
+                            | ExprAbort _ => result_t
+                            | ExprSuccess y => ExprSuccess (x :: y)%list
+                            end)
+             end
+     end eq_refl
+   in match e as e' return e = e' -> _ with
+   | Const val => fun _ => (world, ExprSuccess val)
+   | LocalVar name => fun _ =>
+       (world, match map_lookup loc name with
+               | Some val => ExprSuccess val
+               | None => expr_error "Local variable not found"
+               end)
+   | StorageVar name => fun _ => 
+       (world, match storage_lookup world name with
+               | Some val => ExprSuccess val
+               | None => expr_error "Storage variable not found"
+               end)
+   | UnOp op a => fun E =>
+       let (world', result) := interpret_expr Ebound fc do_call builtins
+                                              world loc a
+                                              (callset_descend_unop E CallOk)
+       in (world', match result with
+                   | ExprSuccess val => interpret_unop op val
+                   | ExprAbort _ => result
+                   end)
+   | BinOp op a b => fun E =>
+       let (world', result_a) := interpret_expr Ebound fc do_call builtins
+                                                world loc a
+                                                (callset_descend_binop_left E CallOk)
+       in match result_a with
+       | ExprAbort _ => (world', result_a)
+       | ExprSuccess x =>
+         let (world'', result_b) := interpret_expr Ebound fc do_call builtins
+                                                   world' loc b
+                                                   (callset_descend_binop_right E CallOk)
+         in (world'', match result_b with
+                      | ExprAbort _ => result_b
+                      | ExprSuccess y => interpret_binop op x y
+                      end)
+       end
+   | IfThenElse cond yes no => fun E =>
+       let (world', result_cond) := interpret_expr Ebound fc do_call builtins
+                                                   world loc cond
+                                                   (callset_descend_if_cond E CallOk)
+       in match result_cond with
+          | ExprAbort _ => (world', result_cond)
+          | ExprSuccess cond_value =>
+              if (Z_of_uint256 cond_value =? 0)%Z
+                then interpret_expr Ebound fc do_call builtins
+                                    world' loc no
+                                    (callset_descend_if_else E CallOk)
+                else interpret_expr Ebound fc do_call builtins
+                                    world' loc yes
+                                    (callset_descend_if_then E CallOk)
+          end
+   | LogicalAnd a b => fun E =>
+       let (world', result_a) := interpret_expr Ebound fc do_call builtins
+                                                world loc a
+                                                (callset_descend_and_left E CallOk)
+       in match result_a with
+          | ExprAbort _ => (world', result_a)
+          | ExprSuccess a_value =>
+              if (Z_of_uint256 a_value =? 0)%Z
+                then (world', result_a)
+                else interpret_expr Ebound fc do_call builtins
+                                    world' loc b
+                                    (callset_descend_and_right E CallOk)
+          end
+   | LogicalOr a b => fun E =>
+       let (world', result_a) := interpret_expr Ebound fc do_call builtins
+                                                world loc a
+                                                (callset_descend_or_left E CallOk)
+       in match result_a with
+          | ExprAbort msg => (world', result_a)
+          | ExprSuccess a_value =>
+              if (Z_of_uint256 a_value =? 0)%Z
+                then interpret_expr Ebound fc do_call builtins
+                                    world' loc b
+                                    (callset_descend_or_right E CallOk)
+                else (world', result_a)
+          end
+   | PrivateOrBuiltinCall name args => fun E =>
+       let (world', result_args) :=
+         interpret_expr_list world loc args
+                             (callset_descend_args E CallOk)
+       in match result_args with
+          | ExprAbort ab => (world', ExprAbort ab)
+          | ExprSuccess arg_values =>
+              match fun_ctx_descend fc CallOk Ebound E with
+              | Some new_fc => do_call new_fc world' arg_values
+              | None => (* can't resolve the function, maybe it's a builtin *)
+                 match builtins name with
+                 | Some (existT _ arity b) =>
+                    (if (arity =? List.length arg_values)%nat as arity_ok 
+                     return _ = arity_ok -> _
+                         then fun Earity => call_builtin arg_values Earity (b world')
+                         else fun _ => (world', expr_error "builtin with wrong arity"))
+                       eq_refl
+                 | None => (world', expr_error "can't resolve function name")
+                 end
+              end
+          end
+   end eq_refl.
+
+Definition interpret_small_stmt {bigger_call_depth_bound smaller_call_depth_bound: nat}
+                                (Ebound: bigger_call_depth_bound = S smaller_call_depth_bound)
+                                {cd: calldag}
+                                (fc: fun_ctx cd bigger_call_depth_bound)
+                                (do_call: forall
+                                              (fc': fun_ctx cd smaller_call_depth_bound)
+                                              (world: world_state)
+                                              (arg_values: list uint256),
+                                            world_state * expr_result uint256)
+                                (builtins: string -> option builtin)
+                                (world: world_state)
+                                (loc: string_map uint256)
+                                (s: small_stmt)
+                                (CallOk: let _ := string_set_impl in 
+                                         FSet.is_subset (small_stmt_callset s)
+                                                        (decl_callset (fun_decl fc))
+                                         = true)
+: world_state * string_map uint256 * stmt_result uint256
+:= match s as s' return s = s' -> _ with
+   | Pass     => fun _ => (world, loc, StmtSuccess)
+   | Break    => fun _ => (world, loc, StmtAbort AbortBreak)
+   | Continue => fun _ => (world, loc, StmtAbort AbortContinue)
+   | Revert   => fun _ => (world, loc, StmtAbort AbortRevert)
+   | Return None => fun _ => (world, loc, StmtReturnFromFunction zero256)
+   | Return (Some e) => fun E =>
+        let (world', result) := interpret_expr Ebound fc do_call builtins
+                                               world loc e
+                                               (callset_descend_return E CallOk)
+        in (world', loc, match result with
+                         | ExprSuccess value => StmtReturnFromFunction value
+                         | ExprAbort ab => StmtAbort ab
+                         end)
+   | Raise e => fun E =>
+        let (world', result) := interpret_expr Ebound fc do_call builtins
+                                               world loc e
+                                               (callset_descend_raise E CallOk)
+        in (world', loc, StmtAbort (match result with
+                                    | ExprSuccess value => AbortException value
+                                    | ExprAbort ab => ab
+                                    end))
+   | Assert cond maybe_e => fun E =>
+        let (world', result_cond) := interpret_expr Ebound fc do_call builtins
+                                                    world loc cond
+                                                    (callset_descend_assert_cond E CallOk)
+        in match result_cond with
+           | ExprAbort ab => (world', loc, StmtAbort ab)
+           | ExprSuccess value =>
+              if (Z_of_uint256 value =? 0)%Z
+                then match maybe_e as maybe_e' return maybe_e = maybe_e' -> _ with
+                     | None => fun _ => (world', loc, StmtAbort (AbortException zero256))
+                     | Some e => fun Ee =>
+                        let (world'', result_e) :=
+                           interpret_expr Ebound fc do_call builtins
+                                          world loc e
+                                          (callset_descend_assert_error E Ee CallOk)
+                        in match result_e with
+                           | ExprSuccess value =>
+                                              (world'', loc, StmtAbort (AbortException value))
+                           | ExprAbort ab => (world'', loc, StmtAbort ab)
+                           end
+                     end eq_refl
+                else (world', loc, StmtSuccess)
+           end
+   | Assign lhs rhs => fun E =>
+        let (world', result) := interpret_expr Ebound fc do_call builtins
+                                               world loc rhs
+                                               (callset_descend_assign_rhs E CallOk)
+        in do_assign world' loc lhs result
+   | BinOpAssign lhs op rhs => fun E =>
+        let (world', result) := interpret_expr Ebound fc do_call builtins
+                                               world loc rhs
+                                               (callset_descend_binop_assign_rhs E CallOk)
+        in do_binop_assign world' loc lhs op result
+   | ExprStmt e => fun E =>
+                   let (world', result) := 
+                      interpret_expr Ebound fc do_call builtins
+                                            world loc e
+                                            (callset_descend_expr_stmt E CallOk)
+                   in (world', loc, match result with
+                                    | ExprSuccess a => StmtSuccess
+                                    | ExprAbort ab => StmtAbort ab
+                                    end)
+   end eq_refl.
+
+Fixpoint interpret_stmt {bigger_call_depth_bound smaller_call_depth_bound: nat}
+                        (Ebound: bigger_call_depth_bound = S smaller_call_depth_bound)
+                        {cd: calldag}
+                        (fc: fun_ctx cd bigger_call_depth_bound)
+                        (do_call: forall
+                                      (fc': fun_ctx cd smaller_call_depth_bound)
+                                      (world: world_state)
+                                      (arg_values: list uint256),
+                                    world_state * expr_result uint256)
+                        (builtins: string -> option builtin)
+                        (world: world_state)
+                        (loc: string_map uint256)
+                        (s: stmt)
+                        (NotVarDecl: is_local_var_decl s = false)
+                        (CallOk: let _ := string_set_impl in 
+                                 FSet.is_subset (stmt_callset s) 
+                                                (decl_callset (fun_decl fc)) = true)
+{struct s}
+: world_state * string_map uint256 * stmt_result uint256
+:= let fix interpret_stmt_list (world: world_state)
+                               (loc: string_map uint256)
+                               (stmts: list stmt)
+                               (CallOk: let _ := string_set_impl in 
+                                        FSet.is_subset (stmt_list_callset stmts)
+                                                       (decl_callset (fun_decl fc)) = true)
+       {struct stmts}
+       : world_state * string_map uint256 * stmt_result uint256
+       := match stmts as stmts' return stmts = stmts' -> _ with
+          | nil => fun _ => (world, loc, StmtSuccess)
+          | h :: t => fun E =>
+              (if is_local_var_decl h as h_is_var_decl return _ = h_is_var_decl -> _
+                 then fun Evar =>
+                   let name_init := var_decl_unpack h Evar in
+                   let name := fst name_init in
+                   let init := snd name_init in
+                   match map_lookup loc name with
+                   | Some _ => (world, loc, StmtAbort (AbortError "local variable already exists"))
+                   | None =>
+                       match init as init' return init = init' -> _ with
+                       | None => fun _ =>
+                           let '(world', loc', result) :=
+                             interpret_stmt_list world (map_insert loc name zero256) t
+                                                       (callset_descend_stmt_tail E CallOk)
+                           in (world', map_remove loc' name, result)
+                       | Some init_expr => fun Einit =>
+                           let '(world', result) := 
+                                  interpret_expr Ebound fc do_call builtins
+                                                 world loc init_expr
+                                                 (callset_descend_init_expr E Evar Einit CallOk)
+                           in match result with
+                              | ExprSuccess value =>
+                                  let '(world2, loc2, result2) :=
+                                    interpret_stmt_list world (map_insert loc name value) t
+                                                        (callset_descend_stmt_tail E CallOk)
+                                  in (world2, map_remove loc2 name, result2)
+                              | ExprAbort ab => (world', loc, StmtAbort ab)
+                              end
+                       end eq_refl
+                   end
+                 else fun Evar =>
+                   let '(world', loc', result) := 
+                     interpret_stmt Ebound fc do_call builtins
+                                    world loc h Evar
+                                    (callset_descend_stmt_head E CallOk)
+                   in match result with
+                      | StmtSuccess => interpret_stmt_list world' loc' t
+                                                           (callset_descend_stmt_tail E CallOk)
+                      | _ => (world', loc', result)
+                      end) eq_refl
+          end eq_refl
+  in match s as s' return s = s' -> _ with
+  | SmallStmt ss => fun E => interpret_small_stmt Ebound fc do_call builtins
+                                         world loc ss
+                                         (callset_descend_small_stmt E CallOk)
+  | LocalVarDecl _ _ => fun E => False_rect _ (var_decl_helper NotVarDecl E)
+  | IfElseStmt cond yes no => fun E => 
+      let (world', result_cond) := interpret_expr
+                                     Ebound fc do_call builtins
+                                     world loc cond
+                                     (callset_descend_stmt_if_cond E CallOk)
+      in match result_cond with
+         | ExprAbort ab => (world', loc, StmtAbort ab)
+         | ExprSuccess cond_value =>
+             if (Z_of_uint256 cond_value =? 0)%Z
+               then match no as no' return no = no' -> _ with
+                    | None => fun _ => (world', loc, StmtSuccess)
+                    | Some n => fun Eno =>
+                        interpret_stmt_list
+                          world' loc n
+                          (callset_descend_stmt_if_else E Eno CallOk)
+                    end eq_refl
+               else interpret_stmt_list world' loc yes
+                                        (callset_descend_stmt_if_then E CallOk)
+         end
+  | FixedRangeLoop var start stop body => fun E =>
+     let fix interpret_loop_rec (world: world_state)
+                                (loc: string_map uint256)
+                                (cursor: Z)
+                                (countdown: nat)
+          {struct countdown}
+          : world_state * string_map uint256 * stmt_result uint256
+          := match countdown with
+             | O => (world, loc, StmtSuccess)
+             | S new_countdown =>
+                   let loc' := map_insert loc var (uint256_of_Z cursor) in
+                   let '(world', loc'', result) :=
+                          interpret_stmt_list world loc' body
+                                              (callset_descend_fixed_range_loop_body E CallOk)
+                   in match result with
+                      | StmtSuccess | StmtAbort AbortContinue =>
+                          interpret_loop_rec world' loc''
+                                             (Z.succ cursor) new_countdown
+                      | StmtAbort AbortBreak => (world', loc'', StmtSuccess)
+                      | _ => (world', loc'', result)
+                      end
+             end
+     in let start_z := match start with
+                       | Some x => Z_of_uint256 x
+                       | None => 0%Z
+                       end
+     in let stop_z := Z_of_uint256 stop in
+     match map_lookup loc var with
+     | Some _ => (world, loc, StmtAbort (AbortError "loop var already exists"))
+     | None => if (stop_z <=? start_z)%Z
+                 then (* ... with STOP being a greater value than START ...
+                         https://vyper.readthedocs.io/en/stable/control-structures.html#for-loops
+                      *)
+                      (world, loc, StmtAbort (AbortError "empty fixed range loop"))
+                 else let '(world', loc', result) :=
+                             interpret_loop_rec world loc start_z
+                                                (Z.to_nat (stop_z - start_z)%Z)
+                      in (world', map_remove loc' var, result)
+     end
+  | FixedCountLoop var start count body => fun E =>
+     let fix interpret_loop_rec (world: world_state)  (* almost dup from FixedRangeLoop branch *)
+                                (loc: string_map uint256)
+                                (cursor: Z)
+                                (countdown: nat)
+          {struct countdown}
+          : world_state * string_map uint256 * stmt_result uint256
+          := match countdown with
+             | O => (world, loc, StmtSuccess)
+             | S new_countdown =>
+                   let loc' := map_insert loc var (uint256_of_Z cursor) in
+                   let '(world', loc'', result) :=
+                          interpret_stmt_list world loc' body
+                                              (callset_descend_fixed_count_loop_body E CallOk)
+                   in match result with
+                      | StmtSuccess | StmtAbort AbortContinue =>
+                          interpret_loop_rec world' loc''
+                                             (Z.succ cursor) new_countdown
+                      | StmtAbort AbortBreak => (world', loc'', StmtSuccess)
+                      | _ => (world', loc'', result)
+                      end
+             end
+      in match map_lookup loc var with
+         | Some _ => (world, loc, StmtAbort (AbortError "loop var already exists"))
+         | None => let (world', result_start) :=
+                      interpret_expr Ebound fc do_call builtins
+                                     world loc start
+                                     (callset_descend_fixed_count_loop_start E CallOk)
+                   in match result_start with
+                   | ExprAbort ab => (world', loc, StmtAbort ab)
+                   | ExprSuccess start_value =>
+                       let count_z := Z_of_uint256 count in
+                       let count_nat := Z.to_nat count_z in
+                       let start_z := Z_of_uint256 start_value in
+                       let last := (start_z + count_z - 1)%Z in
+                       if (Z_of_uint256 (uint256_of_Z last) =? last)%Z
+                         then
+                           let '(world', loc', result) :=
+                             interpret_loop_rec
+                               world' loc start_z count_nat
+                           in (world', map_remove loc var, result)
+                         else (world, loc, StmtAbort (AbortError "loop range overflows"))
+                   end
+         end
+  end eq_refl.
+
+Fixpoint interpret_stmt_list {bigger_call_depth_bound smaller_call_depth_bound: nat}
+                             (Ebound: bigger_call_depth_bound = S smaller_call_depth_bound)
+                             {cd: calldag}
+                             (fc: fun_ctx cd bigger_call_depth_bound)
+                             (do_call: forall
+                                          (fc': fun_ctx cd smaller_call_depth_bound)
+                                          (world: world_state)
+                                          (arg_values: list uint256),
+                                        world_state * expr_result uint256)
+                             (builtins: string -> option builtin)
+                             (world: world_state) (* XXX this is a huge dup from interpret_stmt! *)
+                             (loc: string_map uint256)
+                             (stmts: list stmt)
+                             (CallOk: let _ := string_set_impl in 
+                                      FSet.is_subset (stmt_list_callset stmts)
+                                                     (decl_callset (fun_decl fc)) = true)
+{struct stmts}
+: world_state * string_map uint256 * stmt_result uint256
+:= match stmts as stmts' return stmts = stmts' -> _ with
+   | nil => fun _ => (world, loc, StmtSuccess)
+   | h :: t => fun E =>
+      (if is_local_var_decl h as h_is_var_decl return _ = h_is_var_decl -> _
+         then fun Evar =>
+           let name_init := var_decl_unpack h Evar in
+           let name := fst name_init in
+           let init := snd name_init in
+           match map_lookup loc name with
+           | Some _ => (world, loc, StmtAbort (AbortError "local variable already exists"))
+           | None =>
+               match init as init' return init = init' -> _ with
+               | None => fun _ =>
+                   let '(world', loc', result) :=
+                     interpret_stmt_list Ebound fc do_call builtins
+                                         world (map_insert loc name zero256) t
+                                         (callset_descend_stmt_tail E CallOk)
+                   in (world', map_remove loc' name, result)
+               | Some init_expr => fun Einit =>
+                   let '(world', result) := 
+                          interpret_expr Ebound fc do_call builtins
+                                         world loc init_expr
+                                         (callset_descend_init_expr E Evar Einit CallOk)
+                   in match result with
+                      | ExprSuccess value =>
+                          let '(world2, loc2, result2) :=
+                            interpret_stmt_list Ebound fc do_call builtins
+                                                world (map_insert loc name value) t
+                                                (callset_descend_stmt_tail E CallOk)
+                          in (world2, map_remove loc2 name, result2)
+                      | ExprAbort ab => (world', loc, StmtAbort ab)
+                      end
+               end eq_refl
+           end
+         else fun Evar =>
+           let '(world', loc', result) := 
+             interpret_stmt Ebound fc do_call builtins
+                            world loc h Evar
+                            (callset_descend_stmt_head E CallOk)
+           in match result with
+              | StmtSuccess => interpret_stmt_list Ebound fc do_call builtins
+                                                   world' loc' t
+                                                   (callset_descend_stmt_tail E CallOk)
+              | _ => (world', loc', result)
+              end) eq_refl
+   end eq_refl.
+
+
 Fixpoint interpret_call {call_depth_bound: nat}
                         {cd: calldag}
                         (builtins: string -> option builtin)
@@ -300,417 +778,17 @@ Fixpoint interpret_call {call_depth_bound: nat}
                         (arg_values: list uint256)
 {struct call_depth_bound}
 : world_state * expr_result uint256
-:= let fix interpret_expr (world: world_state)
-                          (loc: string_map uint256)
-                          (e: expr)
-                          (CallOk: let _ := string_set_impl in 
-                                   FSet.is_subset (expr_callset e)
-                                                  (decl_callset (fun_decl fc))
-                                   = true)
-      {struct e}
-      : world_state * expr_result uint256
-      := let fix interpret_expr_list (world: world_state)
-                                     (loc: string_map uint256)
-                                     (e: list expr)
-                                     (CallOk: let _ := string_set_impl in 
-                                              FSet.is_subset (expr_list_callset e)
-                                                             (decl_callset (fun_decl fc))
-                                              = true)
-            {struct e}
-            : world_state * expr_result (list uint256)
-            := match e as e' return e = e' -> _ with
-               | nil => fun _ => (world, ExprSuccess nil)
-               | (h :: t)%list => fun E =>
-                   let (world', result_h) := interpret_expr world loc h
-                                                            (callset_descend_head E CallOk)
-                   in match result_h with
-                      | ExprAbort ab => (world', ExprAbort ab)
-                      | ExprSuccess x =>
-                         let (world'', result_t) := interpret_expr_list world' loc t
-                                                                        (callset_descend_tail E CallOk)
-                         in (world'', match result_t with
-                                      | ExprAbort _ => result_t
-                                      | ExprSuccess y => ExprSuccess (x :: y)%list
-                                      end)
-                       end
-               end eq_refl
-         in match call_depth_bound as call_depth_bound' return _ = call_depth_bound' -> _ with
-            | O => fun Ebound => False_rect _ (Nat.nlt_0_r (fun_depth fc)
-                                                           (eq_ind _ _ (fun_bound_ok fc) _ Ebound))
-            | S new_call_depth_bound => fun Ebound =>
-
-                 match e as e' return e = e' -> _ with
-                 | Const val => fun _ => (world, ExprSuccess val)
-                 | LocalVar name => fun _ =>
-                     (world, match map_lookup loc name with
-                             | Some val => ExprSuccess val
-                             | None => expr_error "Local variable not found"
-                             end)
-                 | StorageVar name => fun _ => 
-                     (world, match storage_lookup world name with
-                             | Some val => ExprSuccess val
-                             | None => expr_error "Storage variable not found"
-                             end)
-                 | UnOp op a => fun E =>
-                     let (world', result) := interpret_expr world loc a
-                                                            (callset_descend_unop E CallOk)
-                     in (world', match result with
-                                 | ExprSuccess val => interpret_unop op val
-                                 | ExprAbort _ => result
-                                 end)
-                 | BinOp op a b => fun E =>
-                     let (world', result_a) := interpret_expr world loc a
-                                                              (callset_descend_binop_left E CallOk)
-                     in match result_a with
-                     | ExprAbort _ => (world', result_a)
-                     | ExprSuccess x =>
-                       let (world'', result_b) := interpret_expr world' loc b
-                                                                 (callset_descend_binop_right E CallOk)
-                       in (world'', match result_b with
-                                    | ExprAbort _ => result_b
-                                    | ExprSuccess y => interpret_binop op x y
-                                    end)
-                     end
-                 | IfThenElse cond yes no => fun E =>
-                     let (world', result_cond) := interpret_expr world loc cond
-                                                                 (callset_descend_if_cond E CallOk)
-                     in match result_cond with
-                        | ExprAbort _ => (world', result_cond)
-                        | ExprSuccess cond_value =>
-                            if (Z_of_uint256 cond_value =? 0)%Z
-                              then interpret_expr world' loc no
-                                                  (callset_descend_if_else E CallOk)
-                              else interpret_expr world' loc yes
-                                                  (callset_descend_if_then E CallOk)
-                        end
-                 | LogicalAnd a b => fun E =>
-                     let (world', result_a) := interpret_expr world loc a
-                                                              (callset_descend_and_left E CallOk)
-                     in match result_a with
-                        | ExprAbort _ => (world', result_a)
-                        | ExprSuccess a_value =>
-                            if (Z_of_uint256 a_value =? 0)%Z
-                              then (world', result_a)
-                              else interpret_expr world' loc b
-                                                  (callset_descend_and_right E CallOk)
-                        end
-                 | LogicalOr a b => fun E =>
-                     let (world', result_a) := interpret_expr world loc a
-                                                              (callset_descend_or_left E CallOk)
-                     in match result_a with
-                        | ExprAbort msg => (world', result_a)
-                        | ExprSuccess a_value =>
-                            if (Z_of_uint256 a_value =? 0)%Z
-                              then interpret_expr world' loc b
-                                                  (callset_descend_or_right E CallOk)
-                              else (world', result_a)
-                        end
-                 | PrivateOrBuiltinCall name args => fun E =>
-                     let (world', result_args) :=
-                       interpret_expr_list world loc args
-                                           (callset_descend_args E CallOk)
-                     in match result_args with
-                        | ExprAbort ab => (world', ExprAbort ab)
-                        | ExprSuccess arg_values =>
-                            match fun_ctx_descend fc CallOk Ebound E with
-                            | Some new_fc => interpret_call builtins new_fc world' arg_values
-                            | None => (* can't resolve the function, maybe it's a builtin *)
-                               match builtins name with
-                               | Some (existT _ arity b) =>
-                                  (if (arity =? List.length arg_values)%nat as arity_ok 
-                                   return _ = arity_ok -> _
-                                       then fun Earity => call_builtin arg_values Earity (b world')
-                                       else fun _ => (world', expr_error "builtin with wrong arity"))
-                                     eq_refl
-                               | None => (world', expr_error "can't resolve function name")
-                               end
-                            end
-                        end
-                 end eq_refl
-         end eq_refl
-     in let interpret_small_stmt (world: world_state)
-                                 (loc: string_map uint256)
-                                 (s: small_stmt)
-                                 (CallOk: let _ := string_set_impl in 
-                                          FSet.is_subset (small_stmt_callset s)
-                                                         (decl_callset (fun_decl fc))
-                                           =
-                                          true)
-        : world_state * string_map uint256 * stmt_result uint256
-        := match s as s' return s = s' -> _ with
-           | Pass     => fun _ => (world, loc, StmtSuccess)
-           | Break    => fun _ => (world, loc, StmtAbort AbortBreak)
-           | Continue => fun _ => (world, loc, StmtAbort AbortContinue)
-           | Revert   => fun _ => (world, loc, StmtAbort AbortRevert)
-           | Return None => fun _ => (world, loc, StmtReturnFromFunction zero256)
-           | Return (Some e) => fun E =>
-                let (world', result) := interpret_expr world loc e
-                                                       (callset_descend_return E CallOk)
-                in (world', loc, match result with
-                                 | ExprSuccess value => StmtReturnFromFunction value
-                                 | ExprAbort ab => StmtAbort ab
-                                 end)
-           | Raise e => fun E =>
-                let (world', result) := interpret_expr world loc e
-                                                       (callset_descend_raise E CallOk)
-                in (world', loc, StmtAbort (match result with
-                                            | ExprSuccess value => AbortException value
-                                            | ExprAbort ab => ab
-                                            end))
-           | Assert cond maybe_e => fun E =>
-                let (world', result_cond) := interpret_expr world loc cond
-                                                            (callset_descend_assert_cond E CallOk)
-                in match result_cond with
-                   | ExprAbort ab => (world', loc, StmtAbort ab)
-                   | ExprSuccess value =>
-                      if (Z_of_uint256 value =? 0)%Z
-                        then match maybe_e as maybe_e' return maybe_e = maybe_e' -> _ with
-                             | None => fun _ => (world', loc, StmtAbort (AbortException zero256))
-                             | Some e => fun Ee =>
-                                let (world'', result_e) := interpret_expr world loc e
-                                                           (callset_descend_assert_error E Ee CallOk)
-                                in match result_e with
-                                   | ExprSuccess value =>
-                                                      (world'', loc, StmtAbort (AbortException value))
-                                   | ExprAbort ab => (world'', loc, StmtAbort ab)
-                                   end
-                             end eq_refl
-                        else (world', loc, StmtSuccess)
-                   end
-           | Assign lhs rhs => fun E =>
-                let (world', result) := interpret_expr world loc rhs
-                                                       (callset_descend_assign_rhs E CallOk)
-                in do_assign world' loc lhs result
-           | BinOpAssign lhs op rhs => fun E =>
-                let (world', result) := interpret_expr world loc rhs
-                                        (callset_descend_binop_assign_rhs E CallOk)
-                in do_binop_assign world' loc lhs op result
-           | ExprStmt e => fun E =>
-                           let (world', result) := interpret_expr world loc e
-                                                   (callset_descend_expr_stmt E CallOk)
-                           in (world', loc, match result with
-                                            | ExprSuccess a => StmtSuccess
-                                            | ExprAbort ab => StmtAbort ab
-                                            end)
-           end eq_refl
-     in let fix interpret_stmt (world: world_state)
-                               (loc: string_map uint256)
-                               (s: stmt)
-                               (NotVarDecl: is_local_var_decl s = false)
-                               (CallOk: let _ := string_set_impl in 
-                                        FSet.is_subset (stmt_callset s) 
-                                                       (decl_callset (fun_decl fc)) = true)
-           {struct s}
-           : world_state * string_map uint256 * stmt_result uint256
-           := let fix interpret_stmt_list (world: world_state)
-                                          (loc: string_map uint256)
-                                          (stmts: list stmt)
-                                          (CallOk: let _ := string_set_impl in 
-                                                   FSet.is_subset (stmt_list_callset stmts)
-                                                                  (decl_callset (fun_decl fc)) = true)
-                 {struct stmts}
-                 : world_state * string_map uint256 * stmt_result uint256
-                 := match stmts as stmts' return stmts = stmts' -> _ with
-                    | nil => fun _ => (world, loc, StmtSuccess)
-                    | h :: t => fun E =>
-                        (if is_local_var_decl h as h_is_var_decl return _ = h_is_var_decl -> _
-                           then fun Evar =>
-                             let name_init := var_decl_unpack h Evar in
-                             let name := fst name_init in
-                             let init := snd name_init in
-                             match map_lookup loc name with
-                             | Some _ => (world, loc, StmtAbort (AbortError "local variable already exists"))
-                             | None =>
-                                 match init as init' return init = init' -> _ with
-                                 | None => fun _ =>
-                                     let '(world', loc', result) :=
-                                       interpret_stmt_list world (map_insert loc name zero256) t
-                                                                 (callset_descend_stmt_tail E CallOk)
-                                     in (world', map_remove loc' name, result)
-                                 | Some init_expr => fun Einit =>
-                                     let '(world', result) := 
-                                            interpret_expr world loc init_expr
-                                                           (callset_descend_init_expr E Evar Einit CallOk)
-                                     in match result with
-                                        | ExprSuccess value =>
-                                            let '(world2, loc2, result2) :=
-                                              interpret_stmt_list world (map_insert loc name value) t
-                                                                  (callset_descend_stmt_tail E CallOk)
-                                            in (world2, map_remove loc2 name, result2)
-                                        | ExprAbort ab => (world', loc, StmtAbort ab)
-                                        end
-                                 end eq_refl
-                             end
-                           else fun Evar =>
-                             let '(world', loc', result) := 
-                               interpret_stmt world loc h Evar
-                                                    (callset_descend_stmt_head E CallOk)
-                             in match result with
-                                | StmtSuccess => interpret_stmt_list world' loc' t
-                                                                     (callset_descend_stmt_tail E CallOk)
-                                | _ => (world', loc', result)
-                                end) eq_refl
-                    end eq_refl
-          in match s as s' return s = s' -> _ with
-          | SmallStmt ss => fun E => interpret_small_stmt world loc ss
-                                                 (callset_descend_small_stmt E CallOk)
-          | LocalVarDecl _ _ => fun E => False_rect _ (var_decl_helper NotVarDecl E)
-          | IfElseStmt cond yes no => fun E => 
-              let (world', result_cond) := interpret_expr
-                                             world loc cond
-                                             (callset_descend_stmt_if_cond E CallOk)
-              in match result_cond with
-                 | ExprAbort ab => (world', loc, StmtAbort ab)
-                 | ExprSuccess cond_value =>
-                     if (Z_of_uint256 cond_value =? 0)%Z
-                       then match no as no' return no = no' -> _ with
-                            | None => fun _ => (world', loc, StmtSuccess)
-                            | Some n => fun Eno =>
-                                interpret_stmt_list
-                                  world' loc n
-                                  (callset_descend_stmt_if_else E Eno CallOk)
-                            end eq_refl
-                       else interpret_stmt_list world' loc yes
-                                                (callset_descend_stmt_if_then E CallOk)
-                 end
-          | FixedRangeLoop var start stop body => fun E =>
-             let fix interpret_loop_rec (world: world_state)
-                                        (loc: string_map uint256)
-                                        (cursor: Z)
-                                        (countdown: nat)
-                  {struct countdown}
-                  : world_state * string_map uint256 * stmt_result uint256
-                  := match countdown with
-                     | O => (world, loc, StmtSuccess)
-                     | S new_countdown =>
-                           let loc' := map_insert loc var (uint256_of_Z cursor) in
-                           let '(world', loc'', result) :=
-                                  interpret_stmt_list world loc' body
-                                                      (callset_descend_fixed_range_loop_body E CallOk)
-                           in match result with
-                              | StmtSuccess | StmtAbort AbortContinue =>
-                                  interpret_loop_rec world' loc''
-                                                     (Z.succ cursor) new_countdown
-                              | StmtAbort AbortBreak => (world', loc'', StmtSuccess)
-                              | _ => (world', loc'', result)
-                              end
-                     end
-             in let start_z := match start with
-                               | Some x => Z_of_uint256 x
-                               | None => 0%Z
-                               end
-             in let stop_z := Z_of_uint256 stop in
-             match map_lookup loc var with
-             | Some _ => (world, loc, StmtAbort (AbortError "loop var already exists"))
-             | None => if (stop_z <=? start_z)%Z
-                         then (* ... with STOP being a greater value than START ...
-                                 https://vyper.readthedocs.io/en/stable/control-structures.html#for-loops
-                              *)
-                              (world, loc, StmtAbort (AbortError "empty fixed range loop"))
-                         else let '(world', loc', result) :=
-                                     interpret_loop_rec world loc start_z
-                                                        (Z.to_nat (stop_z - start_z)%Z)
-                              in (world', map_remove loc' var, result)
-             end
-          | FixedCountLoop var start count body => fun E =>
-             let fix interpret_loop_rec (world: world_state)  (* almost dup from FixedRangeLoop branch *)
-                                        (loc: string_map uint256)
-                                        (cursor: Z)
-                                        (countdown: nat)
-                  {struct countdown}
-                  : world_state * string_map uint256 * stmt_result uint256
-                  := match countdown with
-                     | O => (world, loc, StmtSuccess)
-                     | S new_countdown =>
-                           let loc' := map_insert loc var (uint256_of_Z cursor) in
-                           let '(world', loc'', result) :=
-                                  interpret_stmt_list world loc' body
-                                                      (callset_descend_fixed_count_loop_body E CallOk)
-                           in match result with
-                              | StmtSuccess | StmtAbort AbortContinue =>
-                                  interpret_loop_rec world' loc''
-                                                     (Z.succ cursor) new_countdown
-                              | StmtAbort AbortBreak => (world', loc'', StmtSuccess)
-                              | _ => (world', loc'', result)
-                              end
-                     end
-              in match map_lookup loc var with
-                 | Some _ => (world, loc, StmtAbort (AbortError "loop var already exists"))
-                 | None => let (world', result_start) :=
-                              interpret_expr world loc start
-                                             (callset_descend_fixed_count_loop_start E CallOk)
-                           in match result_start with
-                           | ExprAbort ab => (world', loc, StmtAbort ab)
-                           | ExprSuccess start_value =>
-                               let count_z := Z_of_uint256 count in
-                               let count_nat := Z.to_nat count_z in
-                               let start_z := Z_of_uint256 start_value in
-                               let last := (start_z + count_z - 1)%Z in
-                               if (Z_of_uint256 (uint256_of_Z last) =? last)%Z
-                                 then
-                                   let '(world', loc', result) :=
-                                     interpret_loop_rec
-                                       world' loc start_z count_nat
-                                   in (world', map_remove loc var, result)
-                                 else (world, loc, StmtAbort (AbortError "loop range overflows"))
-                           end
-                 end
-          end eq_refl
-   in let fix interpret_stmt_list (world: world_state) (* XXX this is a huge dup from interpret_stmt! *)
-                                  (loc: string_map uint256)
-                                  (stmts: list stmt)
-                                  (CallOk: let _ := string_set_impl in 
-                                           FSet.is_subset (stmt_list_callset stmts)
-                                                          (decl_callset (fun_decl fc)) = true)
-         {struct stmts}
-         : world_state * string_map uint256 * stmt_result uint256
-         := match stmts as stmts' return stmts = stmts' -> _ with
-            | nil => fun _ => (world, loc, StmtSuccess)
-            | h :: t => fun E =>
-                (if is_local_var_decl h as h_is_var_decl return _ = h_is_var_decl -> _
-                   then fun Evar =>
-                     let name_init := var_decl_unpack h Evar in
-                     let name := fst name_init in
-                     let init := snd name_init in
-                     match map_lookup loc name with
-                     | Some _ => (world, loc, StmtAbort (AbortError "local variable already exists"))
-                     | None =>
-                         match init as init' return init = init' -> _ with
-                         | None => fun _ =>
-                             let '(world', loc', result) :=
-                               interpret_stmt_list world (map_insert loc name zero256) t
-                                                         (callset_descend_stmt_tail E CallOk)
-                             in (world', map_remove loc' name, result)
-                         | Some init_expr => fun Einit =>
-                             let '(world', result) := 
-                                    interpret_expr world loc init_expr
-                                                   (callset_descend_init_expr E Evar Einit CallOk)
-                             in match result with
-                                | ExprSuccess value =>
-                                    let '(world2, loc2, result2) :=
-                                      interpret_stmt_list world (map_insert loc name value) t
-                                                          (callset_descend_stmt_tail E CallOk)
-                                    in (world2, map_remove loc2 name, result2)
-                                | ExprAbort ab => (world', loc, StmtAbort ab)
-                                end
-                         end eq_refl
-                     end
-                   else fun Evar =>
-                     let '(world', loc', result) := 
-                       interpret_stmt world loc h Evar
-                                            (callset_descend_stmt_head E CallOk)
-                     in match result with
-                        | StmtSuccess => interpret_stmt_list world' loc' t
-                                                             (callset_descend_stmt_tail E CallOk)
-                        | _ => (world', loc', result)
-                        end) eq_refl
-            end eq_refl
-   in match fun_decl fc as d return _ = d -> _ with
+:= match call_depth_bound as call_depth_bound' return _ = call_depth_bound' -> _ with
+   | O => fun Ebound => False_rect _ (Nat.nlt_0_r (fun_depth fc)
+                                                  (eq_ind _ _ (fun_bound_ok fc) _ Ebound))
+   | S new_call_depth_bound => fun Ebound =>
+      match fun_decl fc as d return _ = d -> _ with
       | FunDecl _ arg_names body => fun E =>
           match bind_args arg_names arg_values with
           | inl err => (world, expr_error err)
           | inr loc =>
-              let '(world', loc', result) := interpret_stmt_list world loc body 
+              let '(world', loc', result) := interpret_stmt_list Ebound fc (interpret_call builtins)
+                                                                 builtins world loc body
                                                                  (interpret_call_helper E)
               in (world', match result with
                           | StmtSuccess => ExprSuccess zero256
@@ -719,7 +797,8 @@ Fixpoint interpret_call {call_depth_bound: nat}
                           end)
           end
       | _ => fun _ => (world, expr_error "a declaration is found but it's not a function")
-      end eq_refl.
+      end eq_refl
+  end eq_refl.
 
 Local Lemma make_fun_ctx_helper {cd: calldag}
                           {name: string}
